memabs/SemDef.v
@@ -1,0 +1,203 @@
+Require Import Coqlib.
+Require Import LanguageInterface Events Globalenvs Values Memory AST Errors Smallstep.
+Require Import Clight Ctypes Cop.
+Require Import Coherence CompCertSem Bigstep.
+
+(* Define a language interface with memory abstracted out *)
+Record d_query :=
+  dq {
+      dq_vf: val;
+      dq_sg: signature;
+      dq_args: list val;
+    }.
+Record d_reply :=
+  dr {
+      dr_retval: val;
+    }.
+Canonical Structure li_d :=
+  {|
+  query := d_query;
+  reply := d_reply;
+  entry := dq_vf;
+  |}.
+Inductive q_rel: query li_d -> query li_c -> mem -> Prop:=
+| q_rel_intro:
+    forall vf sg args m,
+      q_rel ({|dq_vf:=vf;dq_sg:=sg;dq_args:=args|})
+            ({|cq_vf:=vf;cq_sg:=sg;cq_args:=args;cq_mem:=m|}) m.
+Inductive r_rel: reply li_d -> reply li_c -> mem -> Prop:=
+  r_rel_intro:
+    forall ret m,
+      r_rel ({|dr_retval:=ret|})
+            ({|cr_retval:=ret;cr_mem:=m|}) m.
+Inductive qr_rel_list: list (query li_d * reply li_d) -> list (query li_c * reply li_c) -> Prop:=
+| qr_rel_nil: qr_rel_list nil nil
+| qr_rel_cons:
+    forall dq dr cq cr ds cs m m',
+      q_rel dq cq m ->
+      r_rel dr cr m' ->
+      qr_rel_list ds cs ->
+      qr_rel_list ((dq, dr)::ds) ((cq, cr)::cs).
+Inductive li_rel: (query li_d * reply li_d) -> (query li_c * reply li_c) -> Prop:=
+| rel_intro:
+    forall vf sg args ret m,
+      li_rel ({|dq_vf:=vf;dq_sg:=sg;dq_args:=args|}, {|dr_retval:=ret|})
+             ({|cq_vf:=vf;cq_sg:=sg;cq_args:=args;cq_mem:=m|}, {|cr_retval:=ret;cr_mem:=m|}).
+
+Program Definition li_dc: li_d --o li_c :=
+  {|
+  has '(d, c) := li_rel d c
+  |}.
+Next Obligation.
+  destruct d1 as [dq1 dr1]. destruct d2 as [dq2 dr2].
+  destruct c1 as [cq1 cr1]. destruct c2 as [cq2 cr2].
+  intuition.
+  - inv H. inv H0. f_equal. exploit H3. f_equal. inversion 1. auto.
+  - inv H. inv H0. inv H1. auto.
+Defined.
+
+Inductive exec {liA liB: language_interface} (σ: !liA --o !liB): query liB -> list (token liA) -> reply liB -> Prop:=
+| exec_intro: forall t q r,
+    has σ (t, (q, r) :: nil) ->
+    exec σ q t r.
+
+Program Definition next {liA liB: language_interface} (σ : !liA --o !liB) w qx rx : !liA --o !liB :=
+  {|
+  has '(s, t) := has σ (w ++ s, (qx, rx)::t);
+  |}.
+Next Obligation.
+  pose proof (has_coh _ _ _ _ H H0). cbn in H1. clear H H0.
+  intros Ht. edestruct H1 as [Hr Hl].
+  apply (@app_coh liA). apply Ht.
+  split. inversion Hr. subst. apply H5. auto.
+  intro. exploit Hl. f_equal. auto. apply app_inv_head.
+Qed.
+
+Module Abs.
+  Section ABS_SEMANTICS.
+    (* the linked system has type liA ->> liD *)
+    Context {liA liB liC liD: language_interface} (Σ: Genv.symtbl -> !liA --o !liB) (C: semantics liC liD).
+    Variable li_rel: (query liB * reply liB) -> (query liC * reply liC) -> Prop.
+    Variable se: Genv.symtbl.
+
+    Variant state : Type :=
+    | st (s: Smallstep.state C) (σ: !liA --o !liB)
+    (* s and σ constitute the state after the external call *)
+    | ext (s: Smallstep.state C) (t: list (token liA)) (σ: !liA --o !liB).
+
+    Inductive step: state -> trace -> state -> Prop :=
+    | step_internal: forall s s' t σ,
+        Step (C se) s t s' ->
+        step (st s σ) t (st s' σ)
+    | step_at_external: forall s s' qa ra qb rb σ w,
+        Smallstep.at_external (C se) s qb ->
+        Smallstep.after_external (C se) s rb s' ->
+        (* (w, r) may not be the "right" execution. In other words, [next σ w q
+           r] might be empty.  But that's fine because it's still related to s
+           per correctness *)
+        exec σ qa w ra ->
+        (* drop the memory and make a query. take the reply and attach the same
+        memory to it *)
+        (* this can be further refined by giving the reply a new memory as long
+        as it's larger than the old one *)
+        li_rel (qa, ra) (qb, rb) ->
+        step (st s σ) E0 (ext s' w (next σ w qa ra))
+    | step_after_external: forall s σ,
+        step (ext s nil σ) E0 (st s σ).
+
+    Inductive initial_state: query liD -> state -> Prop :=
+    | initial_state_intro: forall q s,
+        Smallstep.initial_state (C se) q s ->
+        initial_state q (st s (Σ se)).
+
+    Inductive at_external: state -> query liA -> Prop :=
+    | ext_at_external: forall s q r t σ,
+        at_external (ext s ((q, r) :: t) σ) q.
+    Inductive after_external: state -> reply liA -> state -> Prop :=
+    | ext_after_external: forall s q r t σ,
+        after_external (ext s ((q, r) :: t) σ) r (ext s t σ).
+
+    Inductive final_state: state -> reply liD -> Prop :=
+    | final_state_intro: forall s r σ,
+        Smallstep.final_state (C se) s r ->
+        final_state (st s σ) r.
+
+    Definition lts : lts liA liD state :=
+      {|
+      Smallstep.step _ := step;
+      Smallstep.valid_query := Smallstep.valid_query (C se);
+      Smallstep.initial_state := initial_state;
+      Smallstep.at_external := at_external;
+      Smallstep.after_external := after_external;
+      Smallstep.final_state := final_state;
+      Smallstep.globalenv := Smallstep.globalenv (C se);
+      |}.
+  End ABS_SEMANTICS.
+  Definition semantics {liA liB liC liD: language_interface}
+             skel li_rel (Σ: Genv.symtbl -> !liA --o !liB) (C: Smallstep.semantics liC liD) :=
+    {|
+    Smallstep.skel := skel;
+    Smallstep.activate se := lts Σ C li_rel se;
+    |}.
+  Definition c_semantics sk (C: Clight.program) (Σ: Genv.symtbl -> !li_d --o !li_d) : Smallstep.semantics li_d li_c :=
+    semantics sk li_rel Σ (semantics1 C).
+End Abs.
+
+Module Impl.
+  Section IMPL_SEMANTICS.
+    Context {liA liB liC: language_interface} (σ: Genv.symtbl -> !liA --o liB) (C: semantics liB liC).
+    Variable se: Genv.symtbl.
+
+    Variant state :=
+    | st (s: Smallstep.state C)
+    | ext (s: Smallstep.state C) (t: list (token liA)).
+
+    Inductive step: state -> trace -> state -> Prop :=
+    | step_internal: forall s s' t,
+        Step (C se) s t s' ->
+        step (st s) t (st s')
+    | step_at_external: forall s s' q r t,
+        Smallstep.at_external (C se) s q ->
+        Smallstep.after_external (C se) s r s' ->
+        has (σ se) (t, (q, r)) ->
+        step (st s) E0 (ext s' t)
+    | step_after_external: forall s,
+        step (ext s nil) E0 (st s).
+
+    Inductive initial_state: query liC -> state -> Prop :=
+    | initial_state_intro: forall q s,
+        Smallstep.initial_state (C se) q s ->
+        initial_state q (st s).
+
+    Inductive at_external: state -> query liA -> Prop :=
+    | ext_at_external: forall s q r t,
+        at_external (ext s ((q, r) :: t)) q.
+    Inductive after_external: state -> reply liA -> state -> Prop :=
+    | ext_after_external: forall s q r t,
+        after_external (ext s ((q, r) :: t)) r (ext s t).
+
+    Inductive final_state: state -> reply liC -> Prop :=
+    | final_state_intro: forall s r,
+        Smallstep.final_state (C se) s r ->
+        final_state (st s) r.
+
+    Definition lts : lts liA liC state :=
+      {|
+      Smallstep.step _ := step;
+      Smallstep.valid_query := Smallstep.valid_query (C se);
+      Smallstep.initial_state := initial_state;
+      Smallstep.at_external := at_external;
+      Smallstep.after_external := after_external;
+      Smallstep.final_state := final_state;
+      Smallstep.globalenv := Smallstep.globalenv (C se);
+      |}.
+  End IMPL_SEMANTICS.
+  Definition semantics {liA liB liC: language_interface}
+             skel (σ: Genv.symtbl -> !liA --o liB) (C: Smallstep.semantics liB liC) :=
+    {|
+    Smallstep.skel := skel;
+    Smallstep.activate se := lts σ C se;
+    |}.
+  Definition c_semantics sk (C: Clight.program) (p: Clight.program): Smallstep.semantics li_d li_c :=
+    semantics sk (fun se => clight_bigstep p se @ !li_dc) (semantics1 C).
+End Impl.
